Proved progress and preservation without default functions

doc/formalization/Catala.DefaultCalculus.fst
@@ -18,7 +18,7 @@ type lit =
 
 type exp =
   | EVar    : v:var -> exp
-  | EApp    : fn:exp -> arg:exp -> exp
+  | EApp    : fn:exp -> arg:exp -> tau_arg: ty -> exp
   | EAbs    : v:var -> vty:ty -> body:exp -> exp
   | ELit    : l:lit -> exp
   | EIf     : test:exp -> btrue:exp -> bfalse:exp -> exp
@@ -37,26 +37,23 @@ let is_value e =
   match e with
   | EAbs _ _ _
   | ELit _
-  | EDefault (EAbs _ _ _) _ _
     -> true
   | _             -> false
 
-let rec map (#a: Type) (#b: Type) (l:list a) (f: ((x:a{x << l}) -> Tot b)) : Tot (list b)
-  =
-  match l with
-  | [] -> []
-  | a::tl -> f a::map tl f
-
-val subst : var -> exp -> e:exp -> Tot exp (decreases e)
-let rec subst x e e' =
-  match e' with
-  | EVar x' -> if x = x' then e else e'
+let rec subst (x: var) (e_x: exp) (e: exp) : Tot exp (decreases %[e;0]) =
+  match e with
+  | EVar x' -> if x = x' then e_x else e
   | EAbs x' t e1 ->
-      EAbs x' t (if x = x' then e1 else (subst x e e1))
-  | EApp e1 e2 -> EApp (subst x e e1) (subst x e e2)
+      EAbs x' t (if x = x' then e1 else (subst x e_x e1))
+  | EApp e1 e2 tau_arg -> EApp (subst x e_x e1) (subst x e_x e2) tau_arg
   | ELit l -> ELit l
-  | EIf e1 e2 e3 -> EIf (subst x e e1) (subst x e e2) (subst x e e3)
-  | EDefault just cond subs -> EDefault (subst x e just) (subst x e cond) (map subs (subst x e))
+  | EIf e1 e2 e3 -> EIf (subst x e_x e1) (subst x e_x e2) (subst x e_x e3)
+  | EDefault ejust econd subs ->
+    EDefault (subst x e_x ejust) (subst x e_x econd) (subst_list x e_x subs)
+and subst_list (x: var) (e_x: exp) (subs: list exp)  : Tot (list exp) (decreases %[subs]) =
+  match subs with
+  | [] -> []
+  | hd::tl -> (subst x e_x hd)::(subst_list x e_x tl)
 
 type empty_count_result =
   | AllEmpty
@@ -77,37 +74,41 @@ let rec empty_count (acc: empty_count_result) (l: list exp) : Tot empty_count_re
 
 (**** Stepping judgment *)
 
+let rec map (#a: Type) (#b: Type) (l:list a) (f: ((x:a{x << l}) -> Tot b)) : Tot (list b)
+  =
+  match l with
+  | [] -> []
+  | a::tl -> f a::map tl f
+
+
 let rec step_app
   (e: exp)
   (e1: exp{e1 << e})
   (e2: exp{e2 << e})
+  (tau_arg: ty{tau_arg << e})
     : Tot (option exp)  (decreases %[e; 0]) =
   if is_value e1 then
     match e1 with
     | ELit LConflictError -> Some c_err
     | ELit LEmptyError -> Some e_err
-    | _ ->
+    | _ -> begin
       if is_value e2 then
-        match e1 with
+        (match e1 with
         | EAbs x t e' -> Some (subst x e2 e')
-        | EDefault (EAbs xjust tjust ejust') econs subs -> (* beta_d *)
-          Some (EDefault
-            (subst xjust e2 ejust')
-            (EApp econs e2)
-            (map subs (fun sub -> EApp sub e2)))
-        | _ -> None
+        | _ -> None)
       else
-        match step e2 with
+        (match step e2 with
         | Some (ELit LConflictError) -> Some (ELit LConflictError)
         | Some (ELit LEmptyError) -> Some (ELit LEmptyError)
-        | Some e2' -> Some (EApp e1 e2')
-        | None     -> None
-    else
-      match step e1 with
-      | Some (ELit LConflictError) -> Some c_err
-      | Some (ELit LEmptyError) -> Some e_err
-      | Some e1' -> Some (EApp e1' e2)
-      | None     -> None
+        | Some e2' -> Some (EApp e1 e2' tau_arg)
+        | None     -> None)
+    end
+  else
+    (match step e1 with
+    | Some (ELit LConflictError) -> Some c_err
+    | Some (ELit LEmptyError) -> Some e_err
+    | Some e1' -> Some (EApp e1' e2 tau_arg)
+    | None     -> None)
 
 and step_if
   (e: exp)
@@ -174,10 +175,9 @@ and step_default
     match just with
     | ELit LConflictError -> Some c_err
     | ELit LEmptyError -> Some e_err
-    | ELit _ | EAbs _ _ _ | EDefault (EAbs _ _ _) _ _ -> begin
+    | _ -> begin
       match just, cons with
-      | EAbs _ _ _, EAbs _ _ _
-      |  EDefault (EAbs _ _ _) _ _,  EDefault (EAbs _ _ _) _ _ ->
+      | EAbs _ _ _, EAbs _ _ _ ->
         None
       | ELit LTrue, ELit LEmptyError ->
         Some (EDefault (ELit LFalse) cons subs)
@@ -206,14 +206,14 @@ and step_default
 
 and step (e: exp) : Tot (option exp) (decreases %[e; 5]) =
   match e with
-  | EApp e1 e2 -> step_app e e1 e2
+  | EApp e1 e2 tau_arg -> step_app e e1 e2 tau_arg
   | EIf e1 e2 e3 -> step_if e e1 e2 e3
   | EDefault just cons subs -> step_default e just cons subs
   | _ -> None
 
 (* Testing *)
 let _ =
-  let e0 = EApp (EAbs 0 TBool (EIf (EVar 0) (ELit LFalse) (ELit LTrue))) (ELit LTrue) in
+  let e0 = EApp (EAbs 0 TBool (EIf (EVar 0) (ELit LFalse) (ELit LTrue))) (ELit LTrue) TBool in
   let e1 = EIf (ELit LTrue) (ELit LFalse) (ELit LTrue) in
   let e1' = step e0 in
   assert_norm(e1' == Some e1);
@@ -222,40 +222,41 @@ let _ =
   assert_norm(e2' == Some e2)
 
 (* Testing *)
+(*
 let _ =
   let e0 = EDefault
     (EAbs 0 TBool (EIf (EVar 0) (ELit LTrue) (ELit LFalse)))
     (EAbs 1 TBool (ELit LTrue))
     [ (EAbs 2 TBool (ELit LEmptyError));  (EAbs 3 TBool (ELit LFalse)) ] in
   assert_norm (step e0 == None);
-  let e0 = EApp e0 (ELit LFalse) in
+  let e0 = EApp e0 (ELit LFalse) TBool in
   let e1 = EDefault
     (EIf (ELit LFalse) (ELit LTrue) (ELit LFalse))
-    (EApp (EAbs 1 TBool (ELit LTrue)) (ELit LFalse))
-    [ (EApp (EAbs 2 TBool (ELit LEmptyError)) (ELit LFalse));
-      (EApp (EAbs 3 TBool (ELit LFalse)) (ELit LFalse)) ]
+    (EApp (EAbs 1 TBool (ELit LTrue)) (ELit LFalse) TBool)
+    [ (EApp (EAbs 2 TBool (ELit LEmptyError)) (ELit LFalse) TBool);
+      (EApp (EAbs 3 TBool (ELit LFalse)) (ELit LFalse) TBool) ]
   in
   let e1' = step e0 in (* beta_d *)
   assert_norm(e1' == Some e1);
   let e2 = EDefault
     (ELit LFalse)
-    (EApp (EAbs 1 TBool (ELit LTrue)) (ELit LFalse))
-    [ (EApp (EAbs 2 TBool (ELit LEmptyError)) (ELit LFalse));
-      (EApp (EAbs 3 TBool (ELit LFalse)) (ELit LFalse)) ]
+    (EApp (EAbs 1 TBool (ELit LTrue)) (ELit LFalse) TBool)
+    [ (EApp (EAbs 2 TBool (ELit LEmptyError)) (ELit LFalse) TBool);
+      (EApp (EAbs 3 TBool (ELit LFalse)) (ELit LFalse) TBool) ]
   in
   let e2' = step e1 in (* IfFalse *)
   assert_norm(e2' == Some e2);
   let e3 = EDefault
     (ELit LFalse)
-    (EApp (EAbs 1 TBool (ELit LTrue)) (ELit LFalse))
+    (EApp (EAbs 1 TBool (ELit LTrue)) (ELit LFalse) TBool)
     [ (ELit LEmptyError);
-      (EApp (EAbs 3 TBool (ELit LFalse)) (ELit LFalse)) ]
+      (EApp (EAbs 3 TBool (ELit LFalse)) (ELit LFalse) TBool) ]
   in
   let e3' = step e2 in (* App *)
   assert_norm(e3' == Some e3);
   let e4 = EDefault
     (ELit LFalse)
-    (EApp (EAbs 1 TBool (ELit LTrue)) (ELit LFalse))
+    (EApp (EAbs 1 TBool (ELit LTrue)) (ELit LFalse) TBool)
     [ (ELit LEmptyError);
       (ELit LFalse) ]
   in
@@ -265,6 +266,7 @@ let _ =
   let e5' = step e4 in
   assert_norm(e5' == Some e5); (* DefaultJustifFalseOneSub *)
   ()
+*)
 
 (*** Typing *)
 
@@ -278,285 +280,127 @@ let empty = fun _ -> None
 val extend : env -> var -> ty -> Tot env
 let extend g x t = fun x' -> if x = x' then Some t else g x'
 
-let rec for_all_defaults (subs: list exp) (f: (sub:exp{sub << subs}) -> bool) : bool =
-  match subs with
-  | [] -> true
-  | hd::tl ->
-    if f hd then for_all_defaults tl f else false
-
-/// We extend the types with `TRAny`, that stands for any type in the case of errors
-type tyres =
-  | TRBool  : tyres
-  | TRUnit  : tyres
-  | TRArrow : tin:ty -> tout:tyres -> tyres
-  | TRAny: tyres
-
-let rec ty_to_res (t: ty) : tyres = match t with
-  | TBool -> TRBool
-  | TUnit -> TRUnit
-  | TArrow tin tout -> TRArrow tin (ty_to_res tout)
-
-(**** Unification *)
-
-let rec unify (t1 t2: tyres) : option tyres =
-  match t1, t2 with
-  | TRBool, TRBool
-  | TRUnit, TRUnit -> Some t1
-  | TRAny, TRAny -> Some TRAny
-  | TRAny, t2 -> Some t2
-  | t1, TRAny -> Some t1
-  | TRArrow t11 t12, TRArrow t21 t22 ->
-    if t11 = t21 then
-      match unify t12 t22 with
-      | None -> None
-      | Some t -> Some (TRArrow t11 t)
-    else None
-  | _ -> None
-
-/// Unification is a commutative partial monoïd
-
-let rec unify_comm (t1 t2: tyres)
-    : Lemma (unify t1 t2 == unify t2 t1)
-  =
-  match t1, t2 with
-  | TRArrow t11 t12, TRArrow t21 t22 ->
-    unify_comm t12 t22
-  | _ -> ()
-
-let rec unify_assoc_left (t1 t2 t3: tyres) : Lemma
-    (requires (Some? (unify t2 t3) /\ Some? (unify t1 (Some?.v (unify t2 t3)))))
-    (ensures (
-      Some? (unify t1 t2) /\
-      Some? (unify t1 (Some?.v (unify t2 t3))) /\
-      unify t1 (Some?.v (unify t2 t3)) == unify (Some?.v (unify t1 t2)) t3
-    ))
-    (decreases t3)
-  =
-  match t1, t2, t3 with
-  | TRArrow t11 t12, TRArrow t21 t22, TRArrow t31 t32 ->
-    unify_assoc_left t12 t22 t32
-  | _ -> ()
-
-let rec unify_assoc_right (t1 t2 t3: tyres) : Lemma
-    (requires (Some? (unify t1 t2) /\ Some? (unify (Some?.v (unify t1 t2)) t3)))
-    (ensures (
-      Some? (unify t2 t3) /\
-      Some? (unify (Some?.v (unify t1 t2)) t3) /\
-      unify t1 (Some?.v (unify t2 t3)) == unify (Some?.v (unify t1 t2)) t3
-    ))
-    (decreases t3)
-  =
-  match t1, t2, t3 with
-  | TRArrow t11 t12, TRArrow t21 t22, TRArrow t31 t32 ->
-    unify_assoc_right t12 t22 t32
-  | _ -> ()
-
-
 (**** Typing judgment *)
 
-let rec unify_list (g: env) (subs: list exp) : Tot (option tyres) (decreases %[subs]) =
-  match subs with
-  | [] -> Some TRAny
-  | hd::tl -> begin
-    let unif_tl = unify_list g tl in
-    match unif_tl with
-    | None -> None
-    | Some unif_tl -> begin
-      match typing g hd with
-      | None -> None
-      | Some thd ->
-      unify thd unif_tl
-    end
-  end
+let rec size_tau (tau: ty) : nat =
+  match tau with
+  | TArrow t1 t2 -> 1 + size_tau t1 + size_tau t2
+  | _ -> 1
 
-and typing (g: env) (e: exp) : Tot (option tyres) (decreases %[e; 1]) =
+let rec typing (g: env) (e: exp) (tau: ty) : Tot bool (decreases (e)) =
   match e with
-  | EVar x -> begin
-    match g x with
-    | None -> None
-    | Some t -> Some (ty_to_res t)
-  end
+  | EVar x -> g x = Some tau
   | EAbs x t e1 -> begin
-    match typing (extend g x t) e1 with
-    | Some t' -> Some (TRArrow t t')
-    | None -> None
+    match tau with
+    | TArrow tau_in tau_out ->
+      t = tau_in && typing (extend g x t) e1 tau_out
+    | _ -> false
   end
-  | EApp e1 e2 -> begin
-    match typing g e1, typing g e2 with
-    | Some TRAny, Some t2 ->
-      Some TRAny
-    | Some (TRArrow t11 t12), Some t2 -> unify (ty_to_res t11) t2
-    | _, _ -> None
-  end
-  | ELit LTrue  -> Some TRBool
-  | ELit LFalse -> Some TRBool
-  | EIf e1 e2 e3 -> begin
-    match typing g e1, typing g e2, typing g e3 with
-    | Some TRBool, Some t2, Some t3
-    | Some TRAny, Some t2, Some t3 -> unify t2 t3
-    | _, _, _ -> None
-  end
-  | EDefault (EAbs xjust tjust ejust) (EAbs xcons tcons econs) subs -> begin (* DefaultFun *)
-     if tjust = tcons then
-       match typing (extend g xjust tjust) ejust, typing (extend g xcons tcons) econs with
-       | Some tjust', Some tcons' -> begin
-         match unify tjust' tcons' with
-         | Some tjust' -> begin
-           match unify_list g subs with
-           | None -> None
-           | Some unif_subs -> unify (TRArrow tjust tjust') unif_subs
-         end
-         | None -> None
-       end
-       | _,_ -> None
-     else None
-  end
-  | EDefault tjust tcons subs -> begin (* DefaultBase *)
-    match typing g tjust, typing g tcons with
-    | Some TRBool, Some tcons
-    | Some TRAny, Some tcons -> begin
-      match unify_list g subs with
-      | None -> None
-      | Some unif_subs -> unify tcons unif_subs
-    end
-    | _, _ -> None
-  end
-  | _ -> None
+  | EApp e1 e2 tau_arg ->
+    typing g e1 (TArrow tau_arg tau) && typing g e2 tau_arg
+  | ELit LTrue  -> tau = TBool
+  | ELit LFalse -> tau = TBool
+  | ELit LEmptyError -> true
+  | ELit LConflictError -> true
+  | EIf e1 e2 e3 -> typing g e1 TBool && typing g e2 tau && typing g e3 tau
+  | EDefault ejust econs subs ->
+    (* DefaultBase *)
+    typing g ejust TBool && typing g econs tau &&
+    typing_list g subs tau
+  | _ -> false
+and typing_list (g: env) (subs: list exp) (tau: ty)
+    : Tot bool (decreases (subs))
+  =
+  match subs with
+  | [] -> true
+  | hd::tl -> typing g hd tau && typing_list g tl tau
 
 (*** Progress *)
 
 (**** Progress lemmas *)
 
-let is_bool_value_cannot_be_default_abs (g: env) (e: exp) : Lemma
-    (requires (is_value e /\ (match typing g e with
-      | Some TRAny | Some TRBool -> True
-      | _ -> False
-    ))) (ensures (
+let is_bool_value_cannot_be_abs (g: env) (e: exp) : Lemma
+    (requires (is_value e /\ (typing g e TBool))) (ensures (
       match e with
       | ELit LUnit -> False
       | ELit _ -> True
       | _ -> False
     ))
-  =
-  match e with
-  | ELit _ -> ()
-  | EDefault (EAbs xjust tjust ejust) (EAbs xcons tcons econs) subs -> begin
-    match typing g e with
-    | Some TRAny
-    | Some TRBool ->
-      if tjust = tcons then begin
-        match
-          typing (extend g xjust tjust) ejust,
-          typing (extend g xcons tcons) econs
-        with
-        | Some tjust', Some tcons' -> begin
-          match unify tjust' tcons' with
-          | Some tjust' ->
-            let te = unify_list g subs in
-            assert(typing g e == te)
-          | None -> ()
-         end
-       | _ -> ()
-     end else ()
-     | _ -> ()
-   end
-   | _ -> ()
-
-let rec unify_compose_ok (x y z: tyres) : Lemma
-   (requires (Some? (unify y z) /\ Some? (unify x (Some?.v (unify y z)))))
-   (ensures (Some? (unify x z)))
-   =
-   match x, y, z with
-   | TRArrow x1 x2, TRArrow y1 y2, TRArrow z1 z2 -> unify_compose_ok x2 y2 z2
-   | _ -> ()
+  = ()
 
 #push-options "--fuel 3 --ifuel 2 --z3rlimit 20"
 let typing_conserved_by_list_reduction
   (g: env)
-  (just cons: exp)
   (subs: list exp)
+  (tau: ty)
     : Lemma
       (requires (
-        ~ (EAbs? just /\ EAbs? cons) /\
-        Some? (typing g (EDefault just cons subs))
+        (typing_list g subs tau)
       ))
-      (ensures (Cons? subs ==> Some? (typing g (EDefault just cons (Cons?.tl subs)))))
+      (ensures (Cons? subs ==> (typing_list g (Cons?.tl subs) tau)))
   =
-  match subs with
-  | [] -> ()
-  | hd1::tl ->
-    match typing g just, typing g cons with
-    | Some TRBool, Some tcons
-    | Some TRAny, Some tcons ->
-      let e = EDefault just cons subs in
-      let t_out_sub = unify_list g subs in
-      let thd1 = Some?.v (typing g hd1) in
-      unify_compose_ok tcons thd1 (Some?.v (unify_list g tl))
-    | _ -> ()
+  ()
 #pop-options
 
 (**** Progress theorem *)
 
 #push-options "--fuel 2 --ifuel 1 --z3rlimit 20"
-val progress : e:exp -> Lemma
-      (requires (Some? (typing empty e)))
+let rec progress (e:exp) (tau: ty) : Lemma
+      (requires (typing empty e tau))
       (ensures (is_value e \/ (Some? (step e))))
       (decreases %[e; 3])
-let rec progress e =
+  =
   match e with
-  | EApp e1 e2 ->
-    progress e1; begin match typing empty e1 with
-    | Some TRAny -> if is_value e1 then
-        match e1 with
-        | ELit (LEmptyError) | ELit (LConflictError) -> ()
-        | EDefault just cons subs -> if is_value e2 then () else progress e2
-      else ()
-    | _ -> progress e2
-    end
-  | EIf e1 e2 e3 -> progress e1; progress e2; progress e3;
-    if is_value e1 then is_bool_value_cannot_be_default_abs empty e1 else ()
+  | EApp e1 e2 tau_arg ->
+    progress e1 (TArrow tau_arg tau); progress e2 tau_arg
+  | EIf e1 e2 e3 -> progress e1 TBool; progress e2 tau; progress e3 tau;
+    if is_value e1 then is_bool_value_cannot_be_abs empty e1 else ()
   | EDefault just cons subs ->
-   if is_value e then () else progress_defaults e just cons subs
+   if is_value e then () else progress_defaults e just cons subs tau
   | _ -> ()
 and progress_defaults
   (e: exp)
   (just: exp{just << e})
   (cons: exp{cons << e})
-  (subs: list exp{subs << e}) : Lemma
-    (requires (~ (is_value e) /\ e == EDefault just cons subs /\ Some? (typing empty e)))
+  (subs: list exp{subs << e})
+  (tau: ty) : Lemma
+    (requires (~ (is_value e) /\ e == EDefault just cons subs /\ (typing empty e tau)))
     (ensures (Some? (step_default e just cons subs)))
     (decreases %[e; 2])
   =
-  progress just;
+  progress just TBool;
   if is_value just then begin
-    is_bool_value_cannot_be_default_abs empty just;
+    is_bool_value_cannot_be_abs empty just;
     match just, cons with
     | ELit LTrue, ELit LEmptyError -> ()
-    | ELit LTrue, _ -> progress cons
-    | ELit LFalse, _ -> progress_defaults_just_false e just cons subs
+    | ELit LTrue, _ -> progress cons tau
+    | ELit LFalse, _ -> progress_defaults_just_false e just cons subs tau
+    | ELit LEmptyError, _ | ELit LConflictError, _ -> ()
   end else ()
 and progress_defaults_just_false
   (e: exp)
   (just: exp{just << e})
   (cons: exp{cons << e})
-  (subs: list exp{subs << e}) : Lemma
+  (subs: list exp{subs << e})
+  (tau: ty) : Lemma
     (requires (
       ~ (is_value e) /\ just == ELit LFalse /\
-      e == EDefault (ELit LFalse) cons subs /\ Some? (typing empty e)
+      e == EDefault (ELit LFalse) cons subs /\ (typing empty e tau)
     ))
     (ensures (Some? (step_subdefaults_just_false e just cons subs)))
     (decreases %[e; 1])
   =
   if List.Tot.for_all (fun sub -> is_value sub) subs then () else
-  progress_defaults_left_to_right e just cons subs
+  progress_defaults_left_to_right e just cons subs tau
 and progress_defaults_left_to_right
   (e: exp)
   (just: exp{just << e})
   (cons: exp{cons << e})
-  (subs: list exp{subs << e}) : Lemma
+  (subs: list exp{subs << e})
+  (tau: ty) : Lemma
     (requires (
       ~ (is_value e) /\ just == ELit LFalse /\
-      Some? (typing empty (EDefault just cons subs))
+      (typing empty (EDefault just cons subs) tau)
     ))
     (ensures (Some? (step_subdefaults_left_to_right e just cons subs)))
     (decreases %[e; 0; subs])
@@ -564,12 +408,10 @@ and progress_defaults_left_to_right
   match subs with
   | [] -> ()
   | hd::tl ->
-    progress hd;
+    progress hd tau;
     if is_value hd then begin
-      assert(Some?.v (typing empty just) == TRBool);
-      let tcons = Some?.v (typing empty cons) in
-      typing_conserved_by_list_reduction empty just cons subs;
-      progress_defaults_left_to_right e just cons tl
+      typing_conserved_by_list_reduction empty subs tau;
+      progress_defaults_left_to_right e just cons tl tau
     end else ()
 #pop-options
 
@@ -580,7 +422,7 @@ and progress_defaults_left_to_right
 let rec appears_free_in (x: var) (e: exp) : Tot bool =
   match e with
   | EVar y -> x = y
-  | EApp e1 e2 -> appears_free_in x e1 || appears_free_in x e2
+  | EApp e1 e2 tau_arg -> appears_free_in x e1 || appears_free_in x e2
   | EAbs y _ e1 -> x <> y && appears_free_in x e1
   | EIf e1 e2 e3 ->
       appears_free_in x e1 || appears_free_in x e2 || appears_free_in x e3
@@ -593,36 +435,46 @@ and appears_free_in_list (x: var) (subs: list exp) : Tot bool =
   | [] -> false
   | hd::tl -> appears_free_in x hd || appears_free_in_list x tl
 
-let rec free_in_context (x:int) (e:exp) (g:env) : Lemma
-      (requires (Some? (typing g e)))
+#push-options "--fuel 3 --ifuel 2"
+let rec free_in_context (x:var) (e:exp) (g:env) (tau: ty) : Lemma
+      (requires (typing g e tau))
       (ensures (appears_free_in x e ==> Some? (g x)))
+      (decreases %[e])
   =
   match e with
   | EVar _
   | ELit _ -> ()
-  | EAbs y t e1 -> free_in_context x e1 (extend g y t)
-  | EApp e1 e2 -> free_in_context x e1 g; free_in_context x e2 g
-  | EIf e1 e2 e3 -> free_in_context x e1 g;
-                    free_in_context x e2 g; free_in_context x e3 g
-  | EDefault ejust econs subs ->
-    free_in_context x ejust g;
-    free_in_context x econs g;
-    free_in_context_list x subs g
-and free_in_context_list (x:int) (subs:list exp) (g:env) : Lemma
-      (requires (Some? (unify_list g subs)))
+  | EAbs y t e1 -> begin
+    match tau with
+    | TArrow _ tau_out -> free_in_context x e1 (extend g y t) tau_out
+  end
+  | EApp e1 e2 tau_arg ->
+    free_in_context x e1 g (TArrow tau_arg tau);
+    free_in_context x e2 g tau_arg
+  | EIf e1 e2 e3 -> free_in_context x e1 g TBool;
+                    free_in_context x e2 g tau; free_in_context x e3 g tau
+  | EDefault ejust econs subs -> begin
+    free_in_context x ejust g TBool;
+    free_in_context x econs g tau;
+    free_in_context_list x subs g tau
+  end
+and free_in_context_list (x:int) (subs:list exp) (g:env) (tau: ty) : Lemma
+      (requires (typing_list g subs tau))
       (ensures (appears_free_in_list x subs ==> Some? (g x)))
+      (decreases %[subs])
   =
   match subs with
   | [] -> ()
   | hd::tl ->
-    free_in_context x hd g;
-    free_in_context_list x tl g
+    free_in_context x hd g tau;
+    free_in_context_list x tl g tau
+#pop-options
 
-let typable_empty_closed (x:var) (e:exp) : Lemma
-      (requires (Some? (typing empty e)))
+let typable_empty_closed (x:var) (e:exp) (tau: ty) : Lemma
+      (requires (typing empty e tau))
       (ensures (not(appears_free_in x e)))
-      [SMTPat (appears_free_in x e)]
-   = free_in_context x e empty
+      [SMTPat (appears_free_in x e); SMTPat (typing empty e tau)]
+   = free_in_context x e empty tau
 
 type equal (g1:env) (g2:env) = forall (x:var). g1 x = g2 x
 
@@ -632,145 +484,199 @@ type equalE (e:exp) (g1:env) (g2:env) =
 type equalE_list (subs:list exp) (g1:env) (g2:env) =
   forall (x:var). appears_free_in_list x subs ==> g1 x = g2 x
 
-let rec context_invariance (e:exp) (g:env) (g':env) : Lemma
+#push-options "--fuel 3 --ifuel 2"
+let rec context_invariance (e:exp) (g:env) (g':env) (tau: ty) : Lemma
   (requires (equalE e g g'))
-  (ensures (typing g e == typing g' e))
+  (ensures (typing g e tau <==> typing g' e tau))
+  (decreases %[e])
   =
   match e with
-  | EAbs x t e1 ->
-     context_invariance e1 (extend g x t) (extend g' x t)
-  | EApp e1 e2 ->
-     context_invariance e1 g g';
-     context_invariance e2 g g'
+  | EAbs x t e1 -> begin
+    match tau with
+    | TArrow _ tau_out ->
+      context_invariance e1 (extend g x t) (extend g' x t) tau_out
+    | _ -> ()
+  end
+  | EApp e1 e2 tau_arg ->
+     context_invariance e1 g g' (TArrow tau_arg tau);
+     context_invariance e2 g g' tau_arg
   | EIf e1 e2 e3 ->
-     context_invariance e1 g g';
-     context_invariance e2 g g';
-     context_invariance e3 g g'
-  | EDefault econs ejust subs ->
-     context_invariance ejust g g';
-     context_invariance econs g g';
-     context_invariance_list subs g g'
+     context_invariance e1 g g' TBool;
+     context_invariance e2 g g' tau;
+     context_invariance e3 g g' tau
+  | EDefault ejust econs subs -> begin
+    context_invariance ejust g g' TBool;
+    context_invariance econs g g' tau;
+    context_invariance_list subs g g' tau
+  end
   | _ -> ()
-and context_invariance_list (subs:list exp) (g:env) (g':env) : Lemma
+and context_invariance_list (subs:list exp) (g:env) (g':env) (tau: ty) : Lemma
   (requires (equalE_list subs g g'))
-  (ensures (unify_list g subs == unify_list g' subs))
+  (ensures (typing_list g subs tau <==> typing_list g' subs tau))
+  (decreases %[subs])
   =
   match subs with
   | [] -> ()
   | hd::tl ->
-    context_invariance hd g g';
-    context_invariance_list tl g g'
+    context_invariance hd g g' tau;
+    context_invariance_list tl g g' tau
+#pop-options
 
-let typing_extensional (g:env) (g':env) (e:exp) : Lemma
+let typing_extensional (g:env) (g':env) (e:exp) (tau: ty) : Lemma
   (requires (equal g g'))
-  (ensures (typing g e == typing g' e))
-   = context_invariance e g g'
+  (ensures (typing g e tau <==> typing g' e tau))
+   = context_invariance e g g' tau
 
 (**** Substitution preservation *)
 
-let typing_sync (t1 t2: option tyres) : Tot Type0 =
-  match t1, t2 with
-  | Some t1, Some t2 -> Some? (unify t1 t2)
-  | None, None -> True
-  | _ -> False
-
-let rec equal_means_sync_aux (t1 t2: tyres) : Lemma
-  (requires (t1 == t2))
-  (ensures (typing_sync (Some t1) (Some t2)))
-  =
-  match t1, t2 with
-  | TRArrow t11 t12, TRArrow t21 t22 ->
-    equal_means_sync_aux t12 t22
-  | _ -> ()
-
-let equal_means_sync (t1 t2: option tyres) : Lemma
-  (requires (t1 == t2))
-  (ensures (typing_sync t1 t2))
-  [SMTPat (typing_sync t1 t2)]
-  =
-  match t1, t2 with
-  | Some t1, Some t2 ->
-    equal_means_sync_aux t1 t2
-  | _ -> ()
-
-let has_type (v: exp) (tau: ty) : Tot prop =
-  match typing empty v with
-  | None -> False
-  | Some ty_v_empty -> begin
-    match unify ty_v_empty (ty_to_res tau) with
-    | None -> False
-    | Some _ -> True
-  end
-
-#push-options "--fuel 2 --ifuel 2 --z3rlimit 10"
-let rec substitution_preserves_typing (x:var) (tau: ty) (e:exp) (v:exp) (g:env) : Lemma
-  (requires (has_type v tau /\  Some? (typing (extend g x tau) e)))
-  (ensures (
-    Some? (typing empty v) /\
-    typing_sync (typing g (subst x v e)) (typing (extend g x tau) e)
-  ))
+#push-options "--fuel 1 --ifuel 1 --z3rlimit 10"
+let rec substitution_preserves_typing (x:var) (tau_x: ty) (e:exp) (v:exp) (g:env) (tau: ty)
+    : Lemma
+      (requires (typing empty v tau_x /\ typing (extend g x tau_x) e tau))
+      (ensures (typing g (subst x v e) tau))
+      (decreases %[e])
    =
-  let Some t_x = typing empty v in
-  let gx = extend g x tau in
+  let gx = extend g x tau_x in
   match e with
   | ELit _ -> ()
   | EVar y ->
-     if x=y then
-       context_invariance v empty g
-     else
-       context_invariance e gx g
-  | EApp e1 e2 ->
-     substitution_preserves_typing x tau e1 v g;
-     substitution_preserves_typing x tau e2 v g;
-     let esubst_e1 = subst x v e1 in
-     let tsubst_e1 = Some?.v (typing g esubst_e1) in
-     let text_e1 = Some?.v (typing gx e1) in
-     let esubst_e2 = subst x v e2 in
-     let tsubst_e2 = Some?.v (typing g esubst_e2) in
-     let text_e2 = Some?.v (typing gx e2) in
-     let esubst_e = subst x v (EApp e1 e2) in
-     let tsubst_e = typing g esubst_e in
-     let text_e = typing gx (EApp e1 e2) in
-     assert(esubst_e == EApp esubst_e1 esubst_e2);
-     assert(typing_sync (Some tsubst_e1) (Some text_e1));
-     assert(TRArrow? text_e1 \/ TRAny? text_e1);
-     begin
-       match text_e1 with
-       | TRAny ->  assume(typing_sync tsubst_e text_e)
-       | TRArrow _ _ -> assume(typing_sync tsubst_e text_e)
-     end
+     if x=y then context_invariance v empty g tau
+     else context_invariance e gx g tau
+  | EApp e1 e2 tau_arg ->
+    substitution_preserves_typing x tau_x e1 v g (TArrow tau_arg tau);
+    substitution_preserves_typing x tau_x e2 v g tau_arg
   | EIf e1 e2 e3 ->
-     substitution_preserves_typing x tau e1 v g;
-     substitution_preserves_typing x tau e2 v g;
-     substitution_preserves_typing x tau e3 v g;
-     admit()
-  | EAbs y t_y e1 ->
-     let gxy = extend gx y t_y in
-     let gy = extend g y t_y in
-     if x=y
-     then begin typing_extensional gxy gy e1; admit() end
-     else
-       (let gyx = extend gy x tau in
-        typing_extensional gxy gyx e1;
-        substitution_preserves_typing x tau e1 v gy)
-  | EDefault ejust econs subs -> admit()
+    substitution_preserves_typing x tau_x e1 v g TBool;
+    substitution_preserves_typing x tau_x e2 v g tau;
+    substitution_preserves_typing x tau_x e3 v g tau
+  | EAbs y t_y e1 -> begin
+    match tau with
+    | TArrow tau_in tau_out ->
+      if tau_in = t_y then begin
+        let gxy = extend gx y t_y in
+        let gy = extend g y t_y in
+        if x = y then
+          typing_extensional gxy gy e1 tau_out
+        else begin
+          let gyx = extend gy x tau_x in
+          typing_extensional gxy gyx e1 tau_out;
+          substitution_preserves_typing x tau_x e1 v gy tau_out
+        end
+      end else ()
+    | _ -> ()
+  end
+  | EDefault ejust econs subs ->
+    substitution_preserves_typing x tau_x ejust v g TBool;
+    substitution_preserves_typing x tau_x econs v g tau;
+    substitution_preserves_typing_list x tau_x subs v g tau
+and substitution_preserves_typing_list
+  (x:var) (tau_x: ty) (subs:list exp) (v:exp) (g:env) (tau: ty)
+    : Lemma
+      (requires (typing empty v tau_x /\ typing_list (extend g x tau_x) subs tau))
+      (ensures (typing_list g (subst_list x v subs) tau))
+      (decreases (%[subs]))
+  =
+  match subs with
+  | [] -> ()
+  | hd::tl ->
+    substitution_preserves_typing x tau_x hd v g tau;
+    substitution_preserves_typing_list x tau_x tl v g tau
 #pop-options
 
 (**** Preservation theorem *)
 
-val preservation : e:exp -> Lemma
-  (requires (Some? (typing empty e) /\ Some? (step e) ))
-  (ensures (Some? (step e) /\
-            typing empty (Some?.v (step e)) == typing empty e))
-let rec preservation e =
-  match e with
-  | EApp e1 e2 ->
-     if is_value e1
-     then (if is_value e2
-           then let EAbs x _ ebody = e1 in
-                substitution_preserves_typing x ebody e2 empty
-           else preservation e2)
-     else preservation e1
+let rec empty_count_preserves_type (acc: empty_count_result) (subs: list exp) (g: env) (tau: ty)
+  : Lemma
+    (requires (typing_list g subs tau /\ (match acc with
+      | OneNonEmpty e' -> typing g e' tau
+      | _ -> True
+    )))
+    (ensures (match empty_count acc subs with
+      | OneNonEmpty e' -> typing g e' tau
+      | _ -> True
+    ))
+    (decreases subs)
+  =
+  match subs with
+  | [] -> ()
+  | hd::tl -> begin
+    match (hd, acc) with
+    | ELit (LEmptyError), AllEmpty -> empty_count_preserves_type AllEmpty tl g tau
+    | ELit (LEmptyError), OneNonEmpty e -> empty_count_preserves_type (OneNonEmpty e) tl g tau
+    | _, Conflict -> ()
+    | _, AllEmpty -> empty_count_preserves_type (OneNonEmpty hd) tl g tau
+    | _ -> ()
+  end
 
-  | EIf e1 _ _ ->
-      if not (is_value e1) then preservation e1
+#push-options "--fuel 3 --ifuel 1 --z3rlimit 20"
+let rec preservation (e:exp) (tau: ty) : Lemma
+  (requires (typing empty e tau /\ Some? (step e)))
+  (ensures (typing empty (Some?.v (step e)) tau))
+  (decreases %[e])
+   =
+  match e with
+  | ELit _ -> ()
+  | EVar _ -> ()
+  | EIf e1 e2 e3 ->
+    if not (is_value e1) then preservation e1 TBool
+  | EApp e1 e2 tau_arg ->
+    if is_value e1 then
+      match e1 with
+      | ELit LConflictError | ELit LEmptyError -> ()
+      | _ ->
+        if is_value e2 then
+          match e1 with
+          | EAbs x _ ebody ->
+           substitution_preserves_typing x tau_arg ebody e2 empty tau
+          | _ -> ()
+        else
+          preservation e2 tau_arg
+      else
+        preservation e1 (TArrow tau_arg tau)
+  | EDefault just cons subs ->
+     if not (is_value just) then
+       preservation just TBool
+     else begin match just, cons with
+       | ELit LTrue, _ ->
+         if not (is_value cons) then
+           preservation cons tau
+         else ()
+       | ELit LFalse , _->
+         if List.Tot.for_all (fun sub -> is_value sub) subs then
+           match empty_count AllEmpty subs with
+           | AllEmpty -> ()
+           | OneNonEmpty e' -> empty_count_preserves_type AllEmpty subs empty tau
+           | Conflict -> ()
+         else preservation_subdefaults_left_to_right e just cons subs tau
+       | _ -> ()
+     end
+  | _ -> ()
+and preservation_subdefaults_left_to_right
+  (e: exp)
+  (just:exp{just << e})
+  (cons:exp{cons << e})
+  (subs: list exp{subs << e})
+  (tau: ty)
+    : Lemma
+      (requires (
+        typing empty (EDefault just cons subs) tau /\
+        Some? (step_subdefaults_left_to_right e just cons subs)
+      ))
+      (ensures (
+        Nil? subs \/ typing empty (Some?.v (step_subdefaults_left_to_right e just cons subs)) tau
+      ))
+      (decreases %[subs])
+  =
+  match subs with
+  | [] -> ()
+  | hd::tl ->
+    if is_value hd then begin
+      typing_conserved_by_list_reduction empty subs tau;
+      preservation_subdefaults_left_to_right e just cons tl tau
+    end else begin
+     preservation hd tau;
+     match step hd with
+     | Some (ELit LConflictError) -> ()
+     | Some hd' -> ()
+    end
+#pop-options
